src/wp.v
@@ -1,0 +1,49 @@
+From stdpp Require Import base.
+
+(* TODO comment *)
+
+Definition wp {A} (a : A) (Q : A → Prop) :=
+  Q a.
+
+Lemma wp_conseq {A} (a : A) (Q Q' : A → Prop) :
+  wp a Q →
+  (∀ x, Q x → Q' x) →
+  wp a Q'.
+Proof.
+  unfold wp. eauto.
+Qed.
+
+Lemma wp_ret {A} (a : A) (Q : A → Prop) :
+  Q a ->
+  wp a Q.
+Proof.
+  eauto.
+Qed.
+
+Definition bind {A B} (a : A) (b : A → B) : B :=
+  let x := a in b x.
+
+Lemma wp_bind {A B} (a : A) (b : A → B) (P : A → Prop) (Q : B → Prop) :
+  wp a P →
+  (∀ x, P x → wp (b x) Q) →
+  wp (bind a b) Q.
+Proof.
+  eauto.
+Qed.
+
+Lemma wp_bind_unary {A B} (a : A) (b : A → B) (Q : B → Prop) :
+  wp a (λ x, wp (b x) Q) →
+  wp (bind a b) Q.
+Proof.
+  eauto.
+Qed.
+
+Lemma wp_bind_eq {A B} (a : A) (b : A → B) (Q : B → Prop) :
+  (∀ x, x = a → wp (b x) Q) →
+  wp (bind a b) Q.
+Proof.
+  eauto.
+Qed.
+
+(* TODO [bind] should be inlined away at extraction *)
+Global Opaque wp.
